adjust notation and use everywher

IMLTT/typed/JudgmentsAndRules.lean
@@ -16,167 +16,196 @@ mutual
   -- Γ ctx
   @[aesop unsafe [constructors]]
   inductive IsCtx : Ctx n → Prop where
-    | empty : IsCtx .empty
+    | empty : IsCtx ε
     | extend : IsCtx Γ → IsType Γ A → IsCtx (Γ ⬝ A)
 
   -- Γ ⊢ A type
   @[aesop unsafe [constructors]]
   inductive IsType : Ctx n → Tm n → Prop where
     -- formation rules
-    | unit_form : IsCtx Γ
-                  → IsType Γ 𝟙
-    | empty_form : IsCtx Γ
-                   → IsType Γ 𝟘
-    | pi_form : IsType Γ A → IsType (Γ ⬝ A) B
-                → IsType Γ (.pi A B)
-    | sigma_form : IsType Γ A → IsType (Γ ⬝ A) B
-                   → IsType Γ (.sigma A B)
-    | iden_form : HasType Γ a A → HasType Γ a' A
-                  → IsType Γ (.iden A a a')
-    | univ_form : IsCtx Γ
-                  → IsType Γ 𝒰
-    | univ_elim : HasType Γ A 𝒰
-                  → IsType Γ A
+    | unit_form :
+      IsCtx Γ
+      → IsType Γ 𝟙
+    | empty_form :
+      IsCtx Γ
+      → IsType Γ 𝟘
+    | pi_form :
+      IsType Γ A → IsType (Γ ⬝ A) B
+      → IsType Γ (ΠA;B)
+    | sigma_form :
+      IsType Γ A → IsType (Γ ⬝ A) B
+      → IsType Γ (ΣA;B)
+    | iden_form :
+      HasType Γ a A → HasType Γ a' A
+      → IsType Γ (a ≃[A] a')
+    | univ_form :
+      IsCtx Γ
+      → IsType Γ 𝒰
+    | univ_elim :
+      HasType Γ A 𝒰
+      → IsType Γ A
 
   -- Γ ⊢ a : A
   @[aesop unsafe [constructors]]
   inductive HasType : Ctx n → Tm n → Tm n → Prop where
     -- structural rules
     -- make sure variables of A refer to to same variables of Γ as before with lifting
-    | var : IsType Γ A
-            → HasType (Γ ⬝ A) (.var 0) (weaken (.shift .id) A)
+    | var :
+      IsType Γ A
+      → HasType (Γ ⬝ A) v(0) (A⌊↑ₚidₚ⌋)
     -- | weak : HasType Γ (.var i) A → IsType Γ B
     --          → HasType (Γ ⬝ B) (.var (.succ i)) (weaken A (.shift .id))
     -- intro rules
-    | unit_intro : IsCtx Γ
-                   → HasType Γ .tt 𝟙
-    | pi_intro : HasType (Γ ⬝ A) b B
-                 → HasType Γ (.lam A b) (.pi A B)
-    | sigma_intro : HasType Γ a A → HasType Γ b (substitute_zero a B)
-                    → HasType Γ (.pairSigma a b) (.sigma A B)
-    | iden_intro : HasType Γ a A
-                   → HasType Γ (.refl A a) (.iden A a a)
+    | unit_intro :
+      IsCtx Γ
+      → HasType Γ ⋆ 𝟙
+    | pi_intro :
+      HasType (Γ ⬝ A) b B
+      → HasType Γ (λA;b) (ΠA;B)
+    | sigma_intro :
+      HasType Γ a A → HasType Γ b (B⌈a⌉₁)
+      → HasType Γ (a&b) (ΣA;B)
+    | iden_intro :
+      HasType Γ a A
+      → HasType Γ (A.refl a) (a ≃[A] a)
     -- universe intro
-    | univ_unit : IsCtx Γ
-                  → HasType Γ 𝟙 𝒰
-    | univ_empty : IsCtx Γ
-                   → HasType Γ 𝟘 𝒰
-    | univ_pi : HasType Γ A 𝒰 → HasType (Γ ⬝ A) B 𝒰
-                → HasType Γ (.pi A B) 𝒰
-    | univ_sigma : HasType Γ A 𝒰 → HasType (Γ ⬝ A) B 𝒰
-                   → HasType Γ (.sigma A B) 𝒰
-    | univ_iden : HasType Γ A 𝒰 → HasType Γ a A → HasType Γ a' A
-                  → HasType Γ (.iden A a a') 𝒰
+    | univ_unit :
+      IsCtx Γ
+      → HasType Γ 𝟙 𝒰
+    | univ_empty :
+      IsCtx Γ
+      → HasType Γ 𝟘 𝒰
+    | univ_pi : 
+      HasType Γ A 𝒰 → HasType (Γ ⬝ A) B 𝒰
+      → HasType Γ (ΠA;B) 𝒰
+    | univ_sigma :
+      HasType Γ A 𝒰 → HasType (Γ ⬝ A) B 𝒰
+      → HasType Γ (ΣA;B) 𝒰
+    | univ_iden : 
+      HasType Γ A 𝒰 → HasType Γ a A → HasType Γ a' A
+      → HasType Γ (a ≃[A] a') 𝒰
     -- elimination rules (except univ)
-    | unit_elim : IsType (Γ ⬝ 𝟙) A → HasType Γ a (substitute_zero .tt A)
-                  → HasType Γ b 𝟙
-                  → HasType Γ (.indUnit A b a) (substitute_zero b A)
-    | empty_elim : IsType (Γ ⬝ 𝟘) A → HasType Γ b 𝟘
-                   → HasType Γ (.indEmpty A b) (substitute_zero b A)
-    | pi_elim : HasType Γ f (.pi A B) → HasType Γ a A
-                → HasType Γ (.app f a) (substitute_zero a B)
-    | sigma_elim : HasType Γ p (.sigma A B) → IsType (Γ ⬝ (.sigma A B)) C
-                   → HasType (Γ ⬝ A ⬝ B) c
-                     (substitute ((.weak (.shift (.shift .id))), .pairSigma (.var 1) (.var 0)) C)
-                   → HasType Γ (.indSigma A B C c p) (substitute_zero p C)
-    | iden_elim : IsType (((Γ ⬝ A) ⬝ (weaken (.shift .id) A))
-                    ⬝ (.iden (weaken (.shift (.shift .id)) A) (.var 1) (.var 0))) B
-                  → HasType Γ b (substitute ( .weak .id, a, a, .refl A a) B)
-                  → HasType Γ p (.iden A a a')
-                  → HasType Γ (.j A B b a a' p) (substitute (.weak .id, a, a', p) B)
-    -- conversion
-    | ty_conv : HasType Γ a A → IsEqualType Γ A B
-                → HasType Γ a B
+    | unit_elim :
+      IsType (Γ ⬝ 𝟙) A → HasType Γ a (A⌈⋆⌉₁) → HasType Γ b 𝟙
+      → HasType Γ (.indUnit A b a) (A⌈b⌉₁)
+    | empty_elim :
+      IsType (Γ ⬝ 𝟘) A → HasType Γ b 𝟘
+      → HasType Γ (.indEmpty A b) (A⌈b⌉₁)
+    | pi_elim :
+      HasType Γ f (ΠA;B) → HasType Γ a A
+      → HasType Γ (f◃a) (B⌈a⌉₁)
+    | sigma_elim :
+      HasType Γ p (ΣA;B) → IsType (Γ ⬝ ΣA;B) C → HasType (Γ ⬝ A ⬝ B) c (C⌈(ₛ↑ₚ↑ₚidₚ), v(1)&v(0)⌉)
+      → HasType Γ (.indSigma A B C c p) (C⌈p⌉₁)
+    | iden_elim :
+      IsType (Γ ⬝ A ⬝ A⌊↑ₚidₚ⌋ ⬝ v(1) ≃[A⌊↑ₚ↑ₚidₚ⌋] v(0)) B
+      → HasType Γ b (B⌈(ₛidₚ), a, a, .refl A a⌉)
+      → HasType Γ p (a ≃[A] a')
+      → HasType Γ (.j A B b a a' p) (B⌈(ₛidₚ), a, a', p⌉)
+      -- conversion
+    | ty_conv : 
+      HasType Γ a A → IsEqualType Γ A B
+      → HasType Γ a B
 
   -- Γ ⊢ A ≡ B type
   @[aesop unsafe [constructors]]
   inductive IsEqualType : Ctx n → Tm n → Tm n → Prop where
     -- congruence rules (formation)
-    | unit_form_eq : IsCtx Γ
-                     → IsEqualType Γ 𝟙 𝟙
-    | empty_form_eq : IsCtx Γ
-                      → IsEqualType Γ 𝟘 𝟘
-    | pi_form_eq : IsEqualType Γ A A' → IsEqualType (Γ ⬝ A) B B'
-                   → IsEqualType Γ (.pi A B) (.pi A' B')
-    | sigma_form_eq : IsEqualType Γ A A' → IsEqualType (Γ ⬝ A) B B'
-                      → IsEqualType Γ (.sigma A B) (.sigma A' B')
-    | iden_form_eq : IsEqualType Γ A A' → IsEqualTerm Γ a₁ a₂ A → IsEqualTerm Γ a₃ a₄ A'
-                     → IsEqualType Γ (.iden A a₁ a₃) (.iden A' a₂ a₄)
-    | univ_form_eq : IsCtx Γ
-                     → IsEqualType Γ 𝒰 𝒰
-    | univ_elim_eq : IsEqualTerm Γ A A' 𝒰 → IsEqualType Γ A A'
+    | unit_form_eq :
+      IsCtx Γ
+      → IsEqualType Γ 𝟙 𝟙
+    | empty_form_eq :
+      IsCtx Γ
+      → IsEqualType Γ 𝟘 𝟘
+    | pi_form_eq :
+      IsEqualType Γ A A' → IsEqualType (Γ ⬝ A) B B'
+      → IsEqualType Γ (ΠA;B) (ΠA';B')
+    | sigma_form_eq :
+      IsEqualType Γ A A' → IsEqualType (Γ ⬝ A) B B'
+      → IsEqualType Γ (ΣA;B) (ΣA';B')
+    | iden_form_eq :
+      IsEqualType Γ A A' → IsEqualTerm Γ a₁ a₂ A → IsEqualTerm Γ a₃ a₄ A'
+      → IsEqualType Γ (a₁ ≃[A] a₃) (a₂ ≃[A'] a₄)
+    | univ_form_eq :
+      IsCtx Γ
+      → IsEqualType Γ 𝒰 𝒰
+    | univ_elim_eq :
+      IsEqualTerm Γ A A' 𝒰
+      → IsEqualType Γ A A'
 
   -- Γ ⊢ a ≡ b : A
   @[aesop unsafe [constructors]]
   inductive IsEqualTerm : Ctx n → Tm n → Tm n → Tm n → Prop where
-    | var_eq : IsType Γ A
-                → IsEqualTerm (Γ ⬝ A) (.var 0) (.var 0) (weaken (.shift .id) A)
+    | var_eq :
+      IsType Γ A
+      → IsEqualTerm (Γ ⬝ A) v(0) v(0) (A⌊↑ₚidₚ⌋)
     -- computation rules
-    | unit_comp : IsType (Γ ⬝ 𝟙) A → HasType Γ a (substitute_zero .tt A)
-                  → IsEqualTerm Γ (.indUnit A .tt a) a (substitute_zero .tt A)
-    | pi_comp : HasType (Γ ⬝ A) b B → HasType Γ a A
-                → IsEqualTerm Γ (.app (.lam A b) a) (substitute_zero a b) (substitute_zero a B)
-    | sigma_comp : HasType Γ a A → HasType Γ b (substitute_zero a B)
-                   → IsType (Γ ⬝ (.sigma A B)) C
-                   → HasType (Γ ⬝ A ⬝ B) c (
-                       substitute ((.weak (.shift (.shift .id))), .pairSigma (.var 1) (.var 0)) C
-                     )
-                   → IsEqualTerm Γ (.indSigma A B C c (.pairSigma a b))
-                     (substitute (.weak .id, a, b) c)
-                     (substitute_zero (.pairSigma a b) C)
-    | iden_comp : IsType (((Γ ⬝ A) ⬝ (weaken (.shift .id) A))
-                    ⬝ (.iden (weaken (.shift (.shift .id)) A) (.var 1) (.var 0))) B
-                  → HasType Γ b
-                    (substitute (.weak .id, a, a, (.refl A a)) B)
-                  → HasType Γ a A
-                  → IsEqualTerm Γ (.j A B b a a (.refl A a)) b
-                    (substitute (.weak .id, a, a, (.refl A a)) B)
+    | unit_comp :
+      IsType (Γ ⬝ 𝟙) A → HasType Γ a (A⌈⋆⌉₁) 
+      → IsEqualTerm Γ (.indUnit A ⋆ a) a (A⌈⋆⌉₁)
+    | pi_comp : 
+      HasType (Γ ⬝ A) b B → HasType Γ a A 
+      → IsEqualTerm Γ ((λA; b)◃a) (b⌈a⌉₁) (B⌈a⌉₁)
+    | sigma_comp : 
+      HasType Γ a A → HasType Γ b (B⌈a⌉₁) → IsType (Γ ⬝ ΣA;B) C 
+      → HasType (Γ ⬝ A ⬝ B) c (C⌈(ₛ↑ₚ↑ₚidₚ), v(1)&v(0)⌉) 
+      → IsEqualTerm Γ (.indSigma A B C c (a&b)) (c⌈(ₛidₚ), a, b⌉) (C⌈a&b⌉₁)
+    | iden_comp :
+      IsType (Γ ⬝ A ⬝ A⌊↑ₚidₚ⌋ ⬝ v(1) ≃[A⌊↑ₚ↑ₚidₚ⌋] v(0)) B
+      → HasType Γ b (B⌈(ₛidₚ), a, a, .refl A a⌉)
+      → HasType Γ a A
+      → IsEqualTerm Γ (.j A B b a a (.refl A a)) b (B⌈(ₛidₚ), a, a, .refl A a⌉)
     -- congruence rules (introduction and elimination)
-    | unit_intro_eq : IsCtx Γ
-                      → IsEqualTerm Γ .tt .tt 𝟙
-    | unit_elim_eq : IsEqualType (Γ ⬝ 𝟙) A A' → IsEqualTerm Γ a a' (substitute_zero .tt A)
-                     → IsEqualTerm Γ b b' 𝟙
-                     → IsEqualTerm Γ (.indUnit A b a) (.indUnit A' b' a') (substitute_zero b A)
-    | empty_elim_eq : IsEqualType (Γ ⬝ 𝟘) A A' → IsEqualTerm Γ b b' 𝟘
-                      → IsEqualTerm Γ (.indEmpty A b) (.indEmpty A' b') (substitute_zero b A)
-    | pi_intro_eq : IsEqualTerm (Γ ⬝ A) b b' B
-                    → IsEqualTerm Γ (.lam A b) (.lam A' b') (.pi A B)
-    | pi_elim_eq : IsEqualTerm Γ f f' (.pi A B) → IsEqualTerm Γ a a' A
-                   → IsEqualTerm Γ (.app f a) (.app f' a') (substitute_zero a B)
-    | sigma_intro_eq : IsEqualTerm Γ a a' A → IsEqualTerm Γ b b' (substitute_zero a B)
-                       → IsEqualTerm Γ (.pairSigma a b) (.pairSigma a' b') (.sigma A B)
-    | sigma_elim_eq : IsEqualType Γ (.sigma A B) (.sigma A' B') 
-                      → IsEqualTerm Γ p p' (.sigma A B)
-                      → IsEqualType (Γ ⬝ (.sigma A B)) C C'
-                      → IsEqualTerm (Γ ⬝ A ⬝ B) c c' (
-                          substitute ((.weak (.shift (.shift .id))),
-                                          .pairSigma (.var 1) (.var 0)) C
-                        )
-                      → IsEqualTerm Γ (.indSigma A B C c p) (.indSigma A' B' C' c' p')
-                        (substitute_zero p C)
-    | iden_intro_eq : IsEqualType Γ A A' → IsEqualTerm Γ a a' A
-                      → IsEqualTerm Γ (.refl A a) (.refl A' a') (.iden A a a)
-    | iden_elim_eq : IsEqualType (((Γ ⬝ A) ⬝ (weaken (.shift .id) A)) ⬝ (
-                          .iden (weaken (.shift (.shift .id)) A) (.var 1) (.var 0)
-                        )) B B'
-                     → IsEqualTerm Γ b b' (substitute (.weak .id, a₁, a₁, .refl A a₁) B)
-                     → IsEqualType Γ (.iden A a₁ a₃) (.iden A' a₂ a₄)
-                     → IsEqualTerm Γ p p' (.iden A a₁ a₃)
-                     → IsEqualTerm Γ (.j A B b a₁ a₃ p) (.j A' B' b' a₂ a₄ p')
-                       (substitute (.weak .id, a₁, a₃, p) B)
-    | univ_unit_eq : IsCtx Γ
-                     → IsEqualTerm Γ 𝟙 𝟙 𝒰
-    | univ_empty_eq : IsCtx Γ
-                     → IsEqualTerm Γ 𝟘 𝟘 𝒰
-    | univ_pi_eq : IsEqualTerm Γ A A' 𝒰 → IsEqualTerm (Γ ⬝ A) B B' 𝒰
-                   → IsEqualTerm Γ (.pi A B) (.pi A' B') 𝒰
-    | univ_sigma_eq : IsEqualTerm Γ A A' 𝒰 → IsEqualTerm (Γ ⬝ A) B B' 𝒰
-                   → IsEqualTerm Γ (.sigma A B) (.sigma A' B') 𝒰
-    | univ_iden_eq : IsEqualTerm Γ A A' 𝒰 → IsEqualTerm Γ a₁ a₂ A → IsEqualTerm Γ a₃ a₄ A 
-                     → IsEqualTerm Γ (.iden A a₁ a₃) (.iden A' a₂ a₄) 𝒰
+    | unit_intro_eq :
+      IsCtx Γ
+      → IsEqualTerm Γ ⋆ ⋆ 𝟙
+    | unit_elim_eq :
+      IsEqualType (Γ ⬝ 𝟙) A A' → IsEqualTerm Γ a a' (A⌈⋆⌉₁) → IsEqualTerm Γ b b' 𝟙
+      → IsEqualTerm Γ (.indUnit A b a) (.indUnit A' b' a') (A⌈b⌉₁)
+    | empty_elim_eq :
+      IsEqualType (Γ ⬝ 𝟘) A A' → IsEqualTerm Γ b b' 𝟘 
+      → IsEqualTerm Γ (.indEmpty A b) (.indEmpty A' b') (A⌈b⌉₁)
+    | pi_intro_eq : 
+      IsEqualTerm (Γ ⬝ A) b b' B
+      → IsEqualTerm Γ (λA; b) (λA'; b') (ΠA;B)
+    | pi_elim_eq :
+      IsEqualTerm Γ f f' (ΠA;B) → IsEqualTerm Γ a a' A
+      → IsEqualTerm Γ (f◃a) (f'◃a') (B⌈a⌉₁)
+    | sigma_intro_eq : 
+      IsEqualTerm Γ a a' A → IsEqualTerm Γ b b' (B⌈a⌉₁)
+      → IsEqualTerm Γ (a&b) (a'&b') (ΣA;B)
+    | sigma_elim_eq : 
+      IsEqualType Γ (ΣA;B) (ΣA';B') → IsEqualTerm Γ p p' (ΣA;B) → IsEqualType (Γ ⬝ ΣA;B) C C'
+      → IsEqualTerm (Γ ⬝ A ⬝ B) c c' (C⌈(ₛ↑ₚ↑ₚidₚ), v(1)&v(0)⌉)
+      → IsEqualTerm Γ (.indSigma A B C c p) (.indSigma A' B' C' c' p') (C⌈p⌉₁)
+    | iden_intro_eq : 
+      IsEqualType Γ A A' → IsEqualTerm Γ a a' A
+      → IsEqualTerm Γ (.refl A a) (.refl A' a') (.iden A a a)
+    | iden_elim_eq : 
+      IsEqualType (Γ ⬝ A ⬝ A⌊↑ₚidₚ⌋ ⬝ v(1) ≃[A⌊↑ₚ↑ₚidₚ⌋] v(0)) B B'
+      → IsEqualTerm Γ b b' (B⌈(ₛidₚ), a₁, a₁, .refl A a₁⌉)
+      → IsEqualType Γ (a₁ ≃[A] a₃) (a₂ ≃[A'] a₄)
+      → IsEqualTerm Γ p p' (a₁ ≃[A] a₃) 
+      → IsEqualTerm Γ (.j A B b a₁ a₃ p) (.j A' B' b' a₂ a₄ p') (B⌈(ₛidₚ), a₁, a₃, p⌉)
+    | univ_unit_eq :
+      IsCtx Γ
+      → IsEqualTerm Γ 𝟙 𝟙 𝒰
+    | univ_empty_eq :
+      IsCtx Γ
+      → IsEqualTerm Γ 𝟘 𝟘 𝒰
+    | univ_pi_eq : 
+      IsEqualTerm Γ A A' 𝒰 → IsEqualTerm (Γ ⬝ A) B B' 𝒰
+      → IsEqualTerm Γ (ΠA;B) (ΠA';B') 𝒰
+    | univ_sigma_eq : 
+      IsEqualTerm Γ A A' 𝒰 → IsEqualTerm (Γ ⬝ A) B B' 𝒰 
+      → IsEqualTerm Γ (ΣA;B) (ΣA';B') 𝒰
+    | univ_iden_eq :
+      IsEqualTerm Γ A A' 𝒰 → IsEqualTerm Γ a₁ a₂ A → IsEqualTerm Γ a₃ a₄ A 
+      → IsEqualTerm Γ (a₁ ≃[A] a₃) (a₂ ≃[A'] a₄) 𝒰
     -- conversion
-    | ty_conv_eq : IsEqualTerm Γ a b A → IsEqualType Γ A B
-                   → IsEqualTerm Γ a b B
+    | ty_conv_eq : 
+      IsEqualTerm Γ a b A → IsEqualType Γ A B
+      → IsEqualTerm Γ a b B
 end
 
 postfix:90 " ctx" => IsCtx
