IMLTT/typed/proofs/admissable/Contexts.lean
@@ -10,23 +10,24 @@ import IMLTT.typed.proofs.admissable.Substitution
 
 import aesop
 
-theorem defeq_is_term' : IsEqualTerm Γ a a' A → HasType Γ a' A :=
+theorem defeq_is_term' : 
+    (Γ ⊢ a ≡ a' ∶ A) → Γ ⊢ a' ∶ A :=
   by
     intro haaA
     match haaA with
     | _ => sorry
 
-theorem context_conv_has_type : HasType (Γ ⬝ A) b B → IsEqualType Γ A A'
-                                → HasType (Γ ⬝ A') b B :=
+theorem context_conv_has_type : 
+    (Γ ⬝ A ⊢ b ∶ B) → Γ ⊢ A ≡ A' type → Γ ⬝ A' ⊢ b ∶ B :=
   sorry
 
-theorem context_conv_is_equal_term : IsEqualTerm (Γ ⬝ A) b b' B → IsEqualType Γ A A'
-                             → IsEqualTerm (Γ ⬝ A') b b' B :=
+theorem context_conv_is_equal_term : 
+    (Γ ⬝ A ⊢ b ≡ b' ∶ B) → Γ ⊢ A ≡ A' type → Γ ⬝ A' ⊢ b ≡ b' ∶ B :=
   sorry
 
 -- TODO: try mutual: symm and context conv
 mutual
-  theorem defeq_is_type' : IsEqualType Γ A A' → IsType Γ A' :=
+  theorem defeq_is_type' : Γ ⊢ A ≡ A' type → Γ ⊢ A' type :=
     by
       intro hAA
       match hAA with
@@ -57,8 +58,8 @@ mutual
           apply IsType.univ_elim
           apply defeq_is_term' hAAU
 
-  theorem context_conv_is_equal_type : IsEqualType (Γ ⬝ A) B B' → IsEqualType Γ A A'
-                                       → IsEqualType (Γ ⬝ A') B B' :=
+  theorem context_conv_is_equal_type :
+      Γ ⬝ A ⊢ B ≡ B' type → Γ ⊢ A ≡ A' type → Γ ⬝ A' ⊢ B ≡ B' type :=
     by
       intro hBB
       intro hAA
@@ -112,8 +113,8 @@ end
 --       · sorry -- apply context_conv_is_equal_type_gen hBB' hAA
 --     | _ => sorry
 
-theorem context_conv_is_ctx : IsCtx (Γ ⬝ A) → IsEqualType Γ A A'
-                              → IsCtx (Γ ⬝ A') :=
+theorem context_conv_is_ctx : 
+    Γ ⬝ A ctx → Γ ⊢ A ≡ A' type → Γ ⬝ A' ctx :=
   fun hiCA : IsCtx (Γ ⬝ A) ↦
     fun hAA : IsEqualType Γ A A' ↦
       match hiCA with
@@ -123,8 +124,8 @@ theorem context_conv_is_ctx : IsCtx (Γ ⬝ A) → IsEqualType Γ A A'
           · apply hiC
           · apply defeq_is_type' hAA
 
-theorem context_conv_is_type : IsType (Γ ⬝ A) B → IsEqualType Γ A A'
-                               → IsType (Γ ⬝ A') B :=
+theorem context_conv_is_type :
+    Γ ⬝ A ⊢ B type → Γ ⊢ A ≡ A' type → Γ ⬝ A' ⊢ B type :=
   fun hB : IsType (Γ ⬝ A) B ↦
     fun hAA : IsEqualType Γ A A' ↦
     match hB with
