IMLTT/typed/proofs/boundary/BoundarySubstitutionCtx.lean
@@ -5,6 +5,6 @@ import IMLTT.typed.JudgmentsAndRules
 
 /-# if substiution works, then adding type to context also -/
 
-theorem boundary_subs_type_ctx : IsType Γ (substitute (.extend σ b) A)  → HasType Γ b B
-                                 → IsType (Γ ⬝ B) (substitute (.lift (σ)) A) :=
+theorem boundary_subs_type_ctx : 
+    Γ ⊢ A⌈σ, b⌉ type → (Γ ⊢ b ∶ B) → Γ ⬝ B ⊢ A⌈⇑ₛσ⌉ type :=
   sorry
