IMLTT/untyped/Weakening.lean
@@ -59,7 +59,9 @@ def shift_tm : Tm n → Tm (n + 1)
   | t => weaken (.shift .id) t
 
 notation:max "idₚ" => Weak.id
-prefix:97 "↑ₚ" => Weak.shift -- TODO: change 'associativity' to prevent having to use parenthesis?
+prefix:97 "↑ₚ" => Weak.shift
 prefix:97 "⇑ₚ" => Weak.lift
+infixl:97 "ₙ⇑ₚ" => lift_weak_n
 infixl:96 "ₚ∘ₚ" => comp_weaken
+notation:95 x "⌊" ρ "⌋ᵥ" => weaken_var ρ x
 notation:95 A "⌊" ρ "⌋" => weaken ρ A
